pre_loaded -> preloaded

theories/Core/ProjectionTraces.v
@@ -25,7 +25,7 @@ Context
   .
 
 Definition composite_vlsm_induced_projection j : VLSM message :=
-  pre_loaded_vlsm (IM j) (valid_message_prop X).
+  preloaded_vlsm (IM j) (valid_message_prop X).
 
 Lemma composite_vlsm_induced_projection_is_projection :
   forall j,
@@ -73,7 +73,7 @@ End sec_projections.
 
 (** ** VLSM Projection Traces *)
 
-Section sec_pre_loaded_projection_traces.
+Section sec_preloaded_projection_traces.
 
 Context
   {message : Type}
@@ -85,8 +85,8 @@ Context
 (* The projection of a preloaded finite valid trace remains a preloaded valid trace. *)
 Lemma preloaded_component_projection :
   VLSM_projection
-    (pre_loaded_with_all_messages_vlsm (free_composite_vlsm IM))
-    (pre_loaded_with_all_messages_vlsm (IM j))
+    (preloaded_with_all_messages_vlsm (free_composite_vlsm IM))
+    (preloaded_with_all_messages_vlsm (IM j))
     (composite_project_label IM j) (fun s => s j).
 Proof.
   apply basic_VLSM_projection_preloaded; intro; intros; [.. | done]
@@ -195,7 +195,7 @@ Proof.
   by apply (VLSM_projection_finite_valid_trace_init_to preloaded_component_projection).
 Qed.
 
-Lemma pre_loaded_with_all_messages_projection_input_valid_transition_eq
+Lemma preloaded_with_all_messages_projection_input_valid_transition_eq
   (s1 s2 : composite_state IM)
   (om1 om2 : option message)
   (l : label (free_composite_vlsm IM))
@@ -213,7 +213,7 @@ Proof.
   by apply Eqdep_dec.UIP_dec.
 Qed.
 
-Lemma pre_loaded_with_all_messages_projection_input_valid_transition_neq
+Lemma preloaded_with_all_messages_projection_input_valid_transition_neq
   [s1 s2 : composite_state IM]
   [om1 om2 : option message]
   [l : label (free_composite_vlsm IM)]
@@ -229,7 +229,7 @@ Proof.
   by state_update_simpl.
 Qed.
 
-End sec_pre_loaded_projection_traces.
+End sec_preloaded_projection_traces.
 
 Section sec_projection_traces_membership.
 
@@ -322,11 +322,11 @@ Context
   component <<j>>.
 
   In this section we establish some basic properties for projections, building up
-  to Lemma [proj_pre_loaded_with_all_messages_incl], which guarantees that all
+  to Lemma [proj_preloaded_with_all_messages_incl], which guarantees that all
   [valid_trace]s of <<Xj>> are also [valid_trace]s for the
-  [pre_loaded_with_all_messages_vlsm] associated to the component <<IM j>>.
+  [preloaded_with_all_messages_vlsm] associated to the component <<IM j>>.
   In particular this ensures that the byzantine traces of <<IM j>> include all
-  [valid_trace]s of <<Xj>> (see Lemma [pre_loaded_with_all_messages_alt_eq]).
+  [valid_trace]s of <<Xj>> (see Lemma [preloaded_with_all_messages_alt_eq]).
 
 *)
 
@@ -424,10 +424,10 @@ Qed.
 
 (**
   As a stepping stone towards proving trace inclusion between <<Xj>> and
-  the [pre_loaded_with_all_messages_vlsm] associated to <<IM j>>, we prove that the
+  the [preloaded_with_all_messages_vlsm] associated to <<IM j>>, we prove that the
   [valid_state_message_prop]erty is transferred.
 *)
-Lemma proj_pre_loaded_with_all_messages_valid_state_message_preservation
+Lemma proj_preloaded_with_all_messages_valid_state_message_preservation
   (s : state Xj)
   (om : option message)
   (Hps : valid_state_message_prop Xj s om)
@@ -435,14 +435,14 @@ Lemma proj_pre_loaded_with_all_messages_valid_state_message_preservation
 Proof.
   induction Hps.
   - by apply valid_initial_state_message; [| destruct om].
-  - apply (valid_generated_state_message (pre_loaded_with_all_messages_vlsm (IM j)))
+  - apply (valid_generated_state_message (preloaded_with_all_messages_vlsm (IM j)))
       with s _om _s om l; [done.. | | done].
     by cbn; eapply (projection_valid_implies_valid IM), Hv.
 Qed.
 
 (** We can now finally prove the main result for this section. *)
-Lemma proj_pre_loaded_with_all_messages_incl :
-  VLSM_incl Xj (pre_loaded_with_all_messages_vlsm (IM j)).
+Lemma proj_preloaded_with_all_messages_incl :
+  VLSM_incl Xj (preloaded_with_all_messages_vlsm (IM j)).
 Proof.
   apply (basic_VLSM_incl Xj); intro; intros.
   - done.
@@ -452,12 +452,12 @@ Proof.
 Qed.
 
 Lemma component_projection_to_preloaded :
-  VLSM_projection X (pre_loaded_with_all_messages_vlsm (IM j))
+  VLSM_projection X (preloaded_with_all_messages_vlsm (IM j))
     (composite_project_label IM j) (fun s => s j).
 Proof.
   eapply VLSM_projection_incl_trans.
   - by apply component_projection.
-  - by apply proj_pre_loaded_with_all_messages_incl.
+  - by apply proj_preloaded_with_all_messages_incl.
 Qed.
 
 (**
@@ -495,16 +495,16 @@ Qed.
 
 (**
   Assuming the [component_projection_validator_prop]erty, the component
-  [pre_loaded_with_all_messages_vlsm] is [VLSM_eq]ual (trace-equivalent) with
+  [preloaded_with_all_messages_vlsm] is [VLSM_eq]ual (trace-equivalent) with
   its corresponding [projection_induced_validator].
 *)
-Lemma pre_loaded_with_all_messages_validator_component_proj_eq
+Lemma preloaded_with_all_messages_validator_component_proj_eq
   (Hvalidator : component_projection_validator_prop)
-  : VLSM_eq (pre_loaded_with_all_messages_vlsm (IM j)) Xj.
+  : VLSM_eq (preloaded_with_all_messages_vlsm (IM j)) Xj.
 Proof.
   eapply VLSM_eq_trans;
     [| apply VLSM_eq_sym, pre_composite_vlsm_induced_projection_validator_iff].
-  apply pre_loaded_with_all_messages_validator_proj_eq.
+  apply preloaded_with_all_messages_validator_proj_eq.
   - by apply component_transition_projection_None.
   - by apply component_label_projection_lift.
   - by apply component_state_projection_lift.
@@ -517,10 +517,10 @@ Proof.
     by unfold composite_project_label; cbn; rewrite (decide_True_pi eq_refl).
 Qed.
 
-Definition pre_loaded_with_all_messages_validator_component_proj_incl
+Definition preloaded_with_all_messages_validator_component_proj_incl
   (Hvalidator : component_projection_validator_prop)
-  : VLSM_incl (pre_loaded_with_all_messages_vlsm (IM j)) Xj :=
-  proj1 (pre_loaded_with_all_messages_validator_component_proj_eq Hvalidator).
+  : VLSM_incl (preloaded_with_all_messages_vlsm (IM j)) Xj :=
+  proj1 (preloaded_with_all_messages_validator_component_proj_eq Hvalidator).
 
 End sec_fixed_projection.
 
@@ -665,7 +665,7 @@ Proof.
   apply (VLSM_weak_embedding_input_valid_transition
     (pre_free_lift_to_free_weak_embedding i s Hs)).
   unshelve eapply (VLSM_incl_input_valid_transition
-    (pre_loaded_vlsm_incl (IM i)
+    (preloaded_vlsm_incl (IM i)
       (valid_message_prop (composite_vlsm IM (free_constraint IM)))
       (valid_message_prop (free_composite_vlsm IM)) _)).
   - apply VLSM_incl_valid_message; [| by intro].
