theories/Core/Equivocators/FixedEquivocationSimulation.v
@@ -150,7 +150,7 @@ Lemma fixed_equivocation_replay_has_message
   im s
   (Him :
     can_produce
-    (pre_loaded_with_all_messages_vlsm
+    (preloaded_with_all_messages_vlsm
       (free_composite_vlsm (equivocator_IM (sub_IM IM (elements equivocating)))))
     s im)
   : composite_has_been_sent (equivocator_IM IM)
@@ -190,8 +190,8 @@ Lemma fixed_equivocation_has_replayable_message_prop
     (strong_fixed_equivocation_constraint IM equivocating)
     (equivocators_fixed_equivocations_constraint IM (elements equivocating)).
 Proof.
-  specialize (vlsm_is_pre_loaded_with_False XE) as HeqXE.
-  specialize (vlsm_is_pre_loaded_with_False X) as HeqX.
+  specialize (vlsm_is_preloaded_with_False XE) as HeqXE.
+  specialize (vlsm_is_preloaded_with_False X) as HeqX.
   specialize (equivocators_fixed_equivocations_vlsm_incl_PreFree IM (elements equivocating)) as HinclE.
   intro; intros.
   destruct iom as [im |]; swap 1 2; [| destruct HcX as [Hsent | Hemitted]].
@@ -343,12 +343,12 @@ Proof.
     hypothesis and conclusion is done to fit the applied lemma.
   *)
   assert (no_initial_messages_in_XE :
-    forall m, ~ initial_message_prop (pre_loaded_vlsm XE (fun _ => False)) m).
+    forall m, ~ initial_message_prop (preloaded_vlsm XE (fun _ => False)) m).
   { intros m [[i [[mi Hmi] Him]] | Hseeded]; [| done].
     by elim (no_initial_messages_in_IM i mi).
   }
-  specialize (vlsm_is_pre_loaded_with_False X) as HeqX.
-  specialize (vlsm_is_pre_loaded_with_False XE) as HeqXE.
+  specialize (vlsm_is_preloaded_with_False X) as HeqX.
+  specialize (vlsm_is_preloaded_with_False XE) as HeqXE.
   apply (VLSM_eq_finite_valid_trace_init_to HeqX) in HtrX.
   apply
     (generalized_equivocators_finite_valid_trace_init_to_rev
@@ -405,13 +405,13 @@ Lemma no_equivocating_equivocators_finite_valid_trace_init_to_rev
     finite_trace_last_output trX = finite_trace_last_output tr.
 Proof.
   assert (no_initial_messages_in_XE :
-    forall m, ~ initial_message_prop (pre_loaded_vlsm XE (fun _ => False)) m).
+    forall m, ~ initial_message_prop (preloaded_vlsm XE (fun _ => False)) m).
   {
     intros m [[i [[mi Hmi] Him]] | Hseeded]; [| done].
     by elim (no_initial_messages_in_IM i mi).
   }
-  specialize (vlsm_is_pre_loaded_with_False X) as HeqX.
-  specialize (vlsm_is_pre_loaded_with_False XE) as HeqXE.
+  specialize (vlsm_is_preloaded_with_False X) as HeqX.
+  specialize (vlsm_is_preloaded_with_False XE) as HeqXE.
   apply (VLSM_eq_finite_valid_trace_init_to HeqX) in HtrX.
   apply
     (generalized_equivocators_finite_valid_trace_init_to_rev
